Passing elaborator now, needs docs, tests, and minor refactoring

AmericanCall/AmericanCall.fst
@@ -39,41 +39,41 @@ type assets =
       outstandingAsset: asset; }
 
 // compress a public key
-val compress: publicKey -> cpk `cost` 132
+val compress: publicKey -> cpk `cost` 305
 let compress pk = let open FStar.UInt8 in // 13
     let parity = (Arr.item 32 pk %^ 2uy) +^ 2uy in
-    let aux (i:nat{i < 32}): byte `cost` 0 = ret (Arr.item (31-i) pk) in // 5
-    let! x = Arr.init_pure 32 aux in // 132 // 292
+    let aux (i:nat{i < 32}): byte `cost` 5 = ret (Arr.item (31-i) pk) in // 5
+    let! x = Arr.init_pure 32 aux in // 292
     ret (parity, x)
 
-val getAsset: option (Dict.t data) -> string -> option asset `cost` 130
+val getAsset: option (Dict.t data) -> string -> option asset `cost` 137
 let getAsset dict fieldName = // 7
     dict >!= Dict.tryFind fieldName // 64
          >?= tryString // 2
          >?= Zen.Asset.parse // 64
 
-val getU64: option (Dict.t data) -> string -> option p64 `cost` 66
-let getU64 dict fieldName = // 14
+val getU64: option (Dict.t data) -> string -> option p64 `cost` 79
+let getU64 dict fieldName = // 13
     let! x = dict >!= Dict.tryFind fieldName // 64
                   >?= tryU64 in // 2
     match x with
     | None | Some 0UL -> OT.none
     | Some x -> OT.some (x <: p64)
 
-val getIssuer: option (Dict.t data) -> option cpk `cost` 198
-let getIssuer dict = // 5
+val getIssuer: option (Dict.t data) -> option cpk `cost` 380
+let getIssuer dict = // 9
     dict >!= Dict.tryFind "Issuer" // 64
          >?= tryPublicKey // 2
-         >?= (compress >> OT.liftCost) // 132
+         >?= (compress >> OT.liftCost) // 305
 
-let parseArgs (dict:option (Dict.t data)): result args `cost` 722 =
-    let! baseAsset = getAsset dict "Base" in // 130
-    let! pairAsset = getAsset dict "Pair" in // 130
-    let! strike = getU64 dict "Strike" in // 66
-    let! payout = getU64 dict "Strike" in // 66
-    let! expiry = getU64 dict "Expiry" in // 66
-    let! issuer = getIssuer dict in  // 198
-    let! options = getU64 dict "Options" in  // 66
+let parseArgs (dict:option (Dict.t data)): result args `cost` 1045 = // 75
+    let! baseAsset = getAsset dict "Base" in // 137
+    let! pairAsset = getAsset dict "Pair" in // 137
+    let! strike = getU64 dict "Strike" in // 79
+    let! payout = getU64 dict "Strike" in // 79
+    let! expiry = getU64 dict "Expiry" in // 79
+    let! issuer = getIssuer dict in  // 380
+    let! options = getU64 dict "Options" in  // 79
     match baseAsset, pairAsset, strike, payout, expiry with
     | Some baseAsset, Some pairAsset, Some strike, Some payout, Some expiry ->
         RT.ok ({ baseAsset=baseAsset; pairAsset=pairAsset;
@@ -86,43 +86,39 @@ let parseArgs (dict:option (Dict.t data)): result args `cost` 722 =
     | _, _, _, _, None -> RT.autoFailw "Could not parse Expiry, or Expiry was 0"
 
 // update a hasher with a compressed public key
-val updateCPK: cpk -> Zen.Hash.Sha3.t -> Zen.Hash.Sha3.t `cost` 198
-let updateCPK (parity, x) sha3 =
+val updateCPK: cpk -> Zen.Hash.Sha3.t -> Zen.Hash.Sha3.t `cost` 203
+let updateCPK (parity, x) sha3 = // 5
     Hash.updateByte parity sha3 // 6
     >>= Hash.updateHash x // 192
 
-let hashArgs (args:args{Some? args.issuer}): hash `cost` 1130 =
+let hashArgs (args:args{Some? args.issuer}): hash `cost` 1162 = // 27
     Hash.updateAsset args.baseAsset Hash.empty // 384
     >>= Hash.updateAsset args.pairAsset // 384
     >>= Hash.updateU64 args.strike // 48
     >>= Hash.updateU64 args.payout // 48
     >>= Hash.updateU64 args.expiry // 48
-    >>= updateCPK (Some?.v args.issuer) // 198
+    >>= updateCPK (Some?.v args.issuer) // 203
     >>= Hash.finalize // 20
 
 // returns the option asset and the outstanding asset
-let getAssets ((version, contractHash):contractId)
-              (args:args{Some? args.issuer})
-              : assets `cost` 1342 =
-    let! hashArgs = hashArgs args in // 1130
+val getAssets: contractId -> args:args{Some? args.issuer} -> assets `cost` 1392
+let getAssets (version, contractHash) args = // 18
+    let! hashArgs = hashArgs args in // 1162
     let! hash2Args = Hash.updateHash hashArgs Hash.empty // 192
                      >>= Hash.finalize in // 20
     ret ({ optionAsset      = version, contractHash, hashArgs;
            outstandingAsset = version, contractHash, hash2Args })
 
 // gets a lock from a cpk
-let cpkLock (cpk:cpk): lock `cost` 218 =
-    let! cpkHash = updateCPK cpk Hash.empty // 198
+let cpkLock (cpk:cpk): lock `cost` 231 = // 8
+    let! cpkHash = updateCPK cpk Hash.empty // 203
                    >>= Hash.finalize in //20
     ret (PKLock cpkHash)
 
 // add 2 spends to a tx from the wallet
-let spend2FromWallet (contractID:contractId)
-                     (wallet:wallet)
-                     (s1:spend)
-                     (s2:spend)
-                     (tx:txSkeleton)
-                     : CR.t `cost` (W.size wallet * 256 + 387) =
+val spend2FromWallet: contractId -> w:wallet -> spend -> spend -> txSkeleton
+                      -> CR.t `cost` (W.size w * 256 + 405)
+let spend2FromWallet contractID wallet s1 s2 tx = // 18
     TX.fromWallet s1.asset s1.amount contractID wallet tx // W.size wallet * 128 + 192
     `OT.bind` TX.fromWallet s2.asset s2.amount contractID wallet // W.size wallet * 128 + 192
     >>= CR.ofOptionTxSkel "Could not generate tx from wallet" // 3
@@ -131,17 +127,17 @@ let spend2FromWallet (contractID:contractId)
 // issuing
 //
 
-let issue (tx:txSkeleton) (contractID:contractId) (issuerCPK:cpk) (args:args)
-          : CR.t `cost` 1947 = let open U64 in
+val issue: txSkeleton -> contractId -> cpk -> args -> CR.t `cost` 2070
+let issue tx contractID issuerCPK args = let open U64 in // 60
     // get the amount of collateral available in the tx
     let! collateral = TX.getAvailableTokens args.pairAsset tx in // 64
     // get the issuer's address from their pubkey
-    let! issuerAddress = cpkLock issuerCPK in // 218
+    let! issuerAddress = cpkLock issuerCPK in // 231
     if collateral <> 0UL && collateral %^ args.payout = 0UL then
         // compute the number of options to issue
         let options: p64 = collateral /^ args.payout in
         // get the assetIDs for the option
-        let! assets = getAssets contractID ({args with issuer=Some issuerCPK; // 1342
+        let! assets = getAssets contractID ({args with issuer=Some issuerCPK; // 1392
                                                        options=Some options }) in
         // lock collateral to the contract
         TX.lockToContract args.pairAsset collateral contractID tx // 64
@@ -159,22 +155,24 @@ let issue (tx:txSkeleton) (contractID:contractId) (issuerCPK:cpk) (args:args)
 // exercising
 //
 
-let exercise (tx:txSkeleton) ({timestamp=ts}:context) (contractID:contractId)
-             (senderCPK:cpk) (wallet:wallet) (args:args)
-             : CR.t `cost` (W.size wallet * 256 + 2549) = let open U64 in
-    if Some? args.issuer then begin
-        let! (senderAddress, issuerAddress, assets, options, baseAmount) = begin // 1906
+val exercise: txSkeleton -> context -> contractId -> cpk -> w:wallet -> args
+              -> CR.t `cost` (W.size w * 256 + 2742)
+let exercise tx ({timestamp=ts}) contractID senderCPK wallet args = // 99
+    match args.issuer with
+    | Some _ -> begin
+        let! (senderAddress, issuerAddress, assets, options, baseAmount) = begin // 1982
             // get the sender and issuer's addresses from their pubkeys
-            let! senderAddress = cpkLock senderCPK in // 218
-            let! issuerAddress = cpkLock (Some?.v args.issuer) in // 218
+            let! senderAddress = cpkLock senderCPK in // 231
+            let! issuerAddress = cpkLock (Some?.v args.issuer) in // 231
             // get the assetIDs for the option
-            let! assets = getAssets contractID args in // 1342
+            let! assets = getAssets contractID args in // 1392
             // get the number of options available in the tx
             let! options = TX.getAvailableTokens assets.optionAsset tx in // 64
             // get the amount of the base asset available in the tx
             let! baseAmount = TX.getAvailableTokens args.baseAsset tx in // 64
             ret (senderAddress, issuerAddress, assets, options, baseAmount)
-            end <: (lock ** lock ** assets ** U64.t ** U64.t) `cost` 1906 in
+            end <: (lock ** lock ** assets ** U64.t ** U64.t) `cost` 1982 in
+        let open U64 in
         match options <> 0UL, baseAmount /^ args.strike = options, ts <^ args.expiry with
         | true, true, true -> begin
             let totalPrice = args.strike *%^ options in
@@ -188,53 +186,56 @@ let exercise (tx:txSkeleton) ({timestamp=ts}:context) (contractID:contractId)
                 // lock the payout to the sender
                 >>= TX.lockToAddress args.pairAsset totalPayout senderAddress in // 64
             // add spends from contract wallet
-            tx >>= spend2FromWallet contractID wallet // W.size wallet * 256 + 387
+            tx >>= spend2FromWallet contractID wallet // W.size wallet * 256 + 405
                         ({ asset=args.pairAsset;          amount=totalPayout })
                         ({ asset=assets.outstandingAsset; amount=options     })
-            end <: CR.t `cost` (W.size wallet * 256 + 643)
+            end <: CR.t `cost` (W.size wallet * 256 + 661)
         | false, _, _ -> RT.autoFailw "Must send nonzero number of calls"
         | _, false, _ -> RT.autoFailw "PaymentAmount must be equal to calls * Strike"
         | _, _, false -> RT.autoFailw "Cannot exercise after expiry"
-        end <: CR.t `cost` (W.size wallet * 256 + 2549)
-    else RT.incFailw (W.size wallet * 256 + 2549) "Could not parse Issuer"
+        end <: CR.t `cost` (W.size wallet * 256 + 2643)
+    | None ->
+        RT.incFailw (W.size wallet * 256 + 2643) "Could not parse Issuer"
 
 
 //
 // expiring
 //
 
-let expireTX (tx:txSkeleton) (contractID:contractId)
-            (args:args{Some? args.issuer/\ Some? args.options})
-            (wallet:wallet): CR.t `cost` (W.size wallet * 256 + 2075) =
+val expireTX: txSkeleton -> contractId
+              -> (args:args{Some? args.issuer/\ Some? args.options}) -> w:wallet
+              -> CR.t `cost` (W.size w * 256 + 2197)
+let expireTX tx contractID args wallet = // 41
     let options = Some?.v args.options in
     let totalPayout = U64.checked_mul options args.payout in
     match totalPayout with
-    | Some totalPayout ->
-        let! issuerAddress = cpkLock (Some?.v args.issuer) in // 218
-        let! assets = getAssets contractID args in // 1342
+    | Some totalPayout -> begin
+        let! issuerAddress = cpkLock (Some?.v args.issuer) in // 231
+        let! assets = getAssets contractID args in // 1392
         // destroy the outstandingAssets
         TX.destroy options assets.outstandingAsset tx // 64
         // lock the pair assets to the issuer address
         >>= TX.lockToAddress args.pairAsset totalPayout issuerAddress // 64
         // add outstandingAsset and pairAsset inputs from wallet
-        >>= spend2FromWallet contractID wallet // W.size wallet * 256 + 387
+        >>= spend2FromWallet contractID wallet // W.size wallet * 256 + 405
                 ({ asset=args.pairAsset;          amount=totalPayout })
                 ({ asset=assets.outstandingAsset; amount=options })
+        end <: CR.t `cost` (W.size wallet * 256 + 2156)
     | None ->
         RT.autoFailw "Overflow in calculating total payout. Try again with lower amount"
 
-val expire: txSkeleton -> context -> contractId -> cpk -> wallet:wallet -> args
-            -> CR.t `cost` (W.size wallet * 256 + 2075)
-let expire tx ({timestamp=timestamp}) contractID senderCPK wallet args =
+val expire: txSkeleton -> context -> contractId -> cpk -> w:wallet -> args
+            -> CR.t `cost` (W.size w * 256 + 2220)
+let expire tx ({timestamp=ts}) contractID senderCPK wallet args = // 23
     let issuer = match args.issuer with
                  | Some issuer -> issuer
                  | None -> senderCPK in
-    match U64.(timestamp >^ args.expiry), Some? args.options with
-    | true, true ->
-        expireTX tx contractID ({ args with issuer = Some issuer }) wallet
+    match U64.(ts >^ args.expiry), args.options with
+    | true, Some _ -> // W.size wallet * 256 + 2197
+        expireTX tx contractID ({args with issuer=Some issuer}) wallet
     | false, _ ->
         RT.autoFailw "Cannot close before expiry"
-    | _, false ->
+    | _, None ->
         RT.autoFailw "Could not parse Options"
 
 //
@@ -243,40 +244,43 @@ let expire tx ({timestamp=timestamp}) contractID senderCPK wallet args =
 
 type mainCR (command:string) (wallet:wallet) (n:nat) = CR.t `cost` begin
     n + ( match command with
-          | "Issue" -> 1947
-          | "Exercise" -> W.size wallet * 256 + 2549
-          | "Expire" -> W.size wallet * 256 + 2075
+          | "Issue" -> 2070
+          | "Exercise" -> W.size wallet * 256 + 2742
+          | "Expire" -> W.size wallet * 256 + 2220
           | _ -> 0 ) end
 
-val main: txSkeleton -> context -> contractId -> command:string
-          -> sender -> option data -> wallet:wallet -> option data
-          -> mainCR command wallet 858
-let main tx context contractID command sender msg wallet _ =
-    let aux (args:args) (senderCPK:cpk): mainCR command wallet 0 =
+val main: txSkeleton -> context -> contractId -> command:string -> sender
+          -> option data -> w:wallet -> option data
+          -> mainCR command w 1377
+let main tx context contractID command sender msg wallet _ = // 13
+    let aux (args:args) (senderCPK:cpk): mainCR command wallet 10 = // 10
         match command with
         | "Issue" ->
-            issue tx contractID senderCPK args // 1947
+            issue tx contractID senderCPK args // 2070
             <: mainCR command wallet 0
-        | "Exercise" ->
-            exercise tx context contractID senderCPK wallet args // W.size wallet * 256 + 2549
-        | "Expire" ->
-            expire tx context contractID senderCPK wallet args // W.size wallet * 256 + 2075
-        | _ ->
+        | "Exercise" -> // W.size wallet * 256 + 2742
+            exercise tx context contractID senderCPK wallet args
+        | "Expire" -> // W.size wallet * 256 + 2220
+            expire tx context contractID senderCPK wallet args
+        | _ -> // 0
             RT.failw "Invalid Command" in
-    let args: result args `cost` 726 =
+    let args: result args `cost` 1049 =
         Zen.Data.( msg >!= tryDict) // 4
-        >>= parseArgs in // 722
-    let senderCPK: result cpk `cost` 132 =
+        >>= parseArgs in // 1045
+    let senderCPK: result cpk `cost` 305 =
         match sender with
-        | PK senderPK ->
-            compress senderPK >>= RT.ok // 132
+        | PK senderPK -> // 305
+            compress senderPK >>= RT.ok
         | _ ->
             RT.autoFailw "Sender must be PK" in
-    RT.bind2 args senderCPK aux
+    RT.bind2 args senderCPK aux // 1049 + 305 + 10 + match command with ...
 
-let cf _ _ _ command _ _ wallet _ =
-    ret (858 + ( match command with
-                 | "Issue" -> 2805
-                 | "Exercise" -> W.size wallet * 256 + 3407
-                 | "Expire" -> W.size wallet * 256 + 2933
-                 | _ -> 0 ))
+val cf: txSkeleton -> context -> command:string -> sender -> option data
+        -> w:wallet -> option data
+        -> nat `cost` 12
+let cf _ _ command _ _ wallet _ = // 12
+    ret ( 1377 + begin match command with
+                 | "Issue" -> 2070
+                 | "Exercise" -> W.size wallet * 256 + 2742
+                 | "Expire" -> W.size wallet * 256 + 2220
+                 | _ -> 0 end )
